src/BasicSecurity.v
@@ -1,0 +1,313 @@
+Require Import Prog ProgMonad.
+Require Import Pred.
+Require Import PredCrash.
+Require Import Hoare.
+Require Import Omega.
+Require Import SepAuto.
+Require Import Word.
+Require Import Nomega.
+Require Import NArith.
+Require Import FunctionalExtensionality.
+Require Import List.
+Require Import AsyncDisk.
+Require Import Hashmap.
+Require Import ListUtils.
+Require Import ProofIrrelevance.
+Require Import BasicProg.
+
+Set Implicit Arguments.
+
+(** * Some helpful [prog] combinators and proofs *)
+
+Lemma sync_invariant_possible_sync : forall (F: rawpred) (m: rawdisk),
+    F m ->
+    sync_invariant F ->
+    possible_sync m =p=> F.
+Proof.
+  unfold sync_invariant; eauto.
+Qed.
+
+Hint Resolve sync_invariant_possible_sync.
+
+Definition prog_secure T (p : prog T) (pre : pred) (post : pred) :=
+  forall m1 m2 mp F1 F2 out1 vm hm,
+
+  (F1 * diskIs mp)%pred m1 ->
+  (F2 * diskIs mp)%pred m2 ->
+  pre mp ->
+  exec m1 vm hm p out1 ->
+
+  (exists r m1' m2' vm' hm' mr,
+   out1 = Finished m1' vm' hm' r /\
+   exec m2 vm hm p (Finished m2' vm' hm' r) /\
+   (F1 * diskIs mr)%pred m1' /\
+   (F2 * diskIs mr)%pred m2' /\
+   post mr) \/
+
+  (exists m1' m2' hm' mc,
+   out1 = Crashed _ m1' hm' /\
+   exec m2 vm hm p (Crashed _ m2' hm') /\
+   (F1 * diskIs mc)%pred m1' /\
+   (F2 * diskIs mc)%pred m2').
+
+Theorem read_secure:
+  forall (a:addr),
+  prog_secure (Read a) (exists v, a |+> v)%pred (exists v, a |+> v)%pred.
+Proof.
+  unfold prog_secure; intros.
+  inv_exec.
+  - (* Finished *)
+    left.
+    unfold ptsto_subset in H1; destruct_lift H1.
+    repeat eexists.
+    + econstructor.
+      econstructor.
+      rewrite (diskIs_pred _ H1) in H0.
+      rewrite (diskIs_pred _ H1) in H.
+      eapply ptsto_valid' in H.
+      eapply ptsto_valid' in H0.
+      rewrite H8 in H; inversion H; subst.
+      eauto.
+    + eauto.
+    + eauto.
+    + pred_apply; cancel.
+      eassign (dummy_cur, dummy0); cancel.
+  - (* Failed *)
+    exfalso.
+    rewrite (diskIs_pred _ H1) in H.
+    destruct_lift H.
+    eapply ptsto_subset_valid' in H.
+    repeat deex.
+    congruence.
+  - (* Crashed *)
+    right.
+    repeat eexists; eauto.
+Qed.
+
+Theorem write_secure:
+  forall (a:addr) v,
+  prog_secure (Write a v) (exists v0, a |+> v0)%pred (exists v0, a |+> (v, vsmerge v0))%pred.
+Proof.
+  unfold prog_secure; intros.
+  inv_exec.
+  - (* Finished *)
+    left.
+    unfold ptsto_subset in H1; destruct_lift H1.
+    repeat eexists.
+    + econstructor.
+      econstructor.
+      rewrite (diskIs_pred _ H1) in H0.
+      rewrite (diskIs_pred _ H1) in H.
+      eapply ptsto_valid' in H.
+      eapply ptsto_valid' in H0.
+      rewrite H13 in H; inversion H; subst.
+      eauto.
+    + eapply diskIs_sep_star_upd. 2: eauto.
+      unfold ptsto in H1; intuition eauto.
+    + rewrite diskIs_pred in H; eauto.
+      eapply ptsto_valid' in H.
+      rewrite H13 in H; inversion H; subst.
+      eapply diskIs_sep_star_upd. 2: eauto.
+      unfold ptsto in H1; intuition eauto.
+    + eapply pimpl_apply.
+      2: eapply ptsto_upd.
+      2: pred_apply; cancel.
+      cancel.
+      eassign (v2, x); unfold vsmerge; simpl.
+      eapply incl_refl.
+  - (* Failed *)
+    exfalso.
+    rewrite (diskIs_pred _ H1) in H.
+    destruct_lift H.
+    eapply ptsto_subset_valid' in H.
+    repeat deex.
+    congruence.
+  - (* Crashed *)
+    right.
+    repeat eexists; eauto.
+Qed.
+
+Theorem ret_secure:
+  forall T (x : T),
+  prog_secure (Ret x) emp emp.
+Proof.
+  unfold prog_secure; intros.
+  inv_exec.
+  left.
+  do 6 eexists; intuition.
+  eauto.
+  eauto.
+  eauto.
+Qed.
+
+Theorem bind_secure:
+  forall T1 T2 (p1 : prog T1) (p2 : T1 -> prog T2) pre post1 post2,
+  prog_secure p1 pre post1 ->
+  (forall x, prog_secure (p2 x) post1 post2) ->
+  prog_secure (Bind p1 p2) pre post2.
+Proof.
+  unfold prog_secure; intros.
+  inv_exec.
+  - (* p1 Finished *)
+    specialize (H _ _ _ _ _ _ _ _ H1 H2 H3 H11).
+    intuition; repeat deex; try congruence.
+    inversion H4; subst.
+    specialize (H0 r _ _ _ _ _ _ _ _ H5 H6 H8 H14).
+    intuition; repeat deex.
+    + left.
+      do 6 eexists; intuition eauto.
+    + right.
+      do 4 eexists; intuition eauto.
+  - (* p1 Failed *)
+    specialize (H _ _ _ _ _ _ _ _ H1 H2 H3 H10).
+    intuition; repeat deex; try congruence.
+  - (* p1 Crashed *)
+    specialize (H _ _ _ _ _ _ _ _ H1 H2 H3 H10).
+    intuition; repeat deex; try congruence.
+    right.
+    inversion H4; subst.
+    do 4 eexists; intuition.
+    constructor.
+    eauto.
+    eauto.
+    eauto.
+Qed.
+
+Theorem frame_secure:
+  forall T (p : prog T) pre post F,
+  prog_secure p pre post ->
+  prog_secure p (F * pre)%pred (F * post)%pred.
+Proof.
+  unfold prog_secure; intros.
+  eapply diskIs_sep_star_split in H2; repeat deex; intuition.
+  rewrite H6 in H0.
+  rewrite H6 in H1.
+  apply sep_star_assoc in H0.
+  apply sep_star_assoc in H1.
+  specialize (H _ _ _ _ _ _ _ _ H0 H1 H2 H3).
+  intuition; repeat deex.
+  - left.
+    apply sep_star_assoc in H7.
+    apply sep_star_assoc in H8.
+    rewrite (diskIs_sep_star_combine _ _ H4 H10) in H7; destruct_lift H7.
+    rewrite (diskIs_sep_star_combine _ _ H4 H10) in H8; destruct_lift H8.
+    do 6 eexists; intuition eauto.
+  - right.
+    apply sep_star_assoc in H7.
+    apply sep_star_assoc in H9.
+    assert ((diskIs mc) mc) by congruence.
+    rewrite (diskIs_sep_star_combine _ _ H4 H5) in H7; destruct_lift H7.
+    rewrite (diskIs_sep_star_combine _ _ H4 H5) in H9; destruct_lift H9.
+    do 4 eexists; intuition eauto.
+Qed.
+
+Theorem pimpl_secure:
+  forall T (p : prog T) pre pre' post post',
+  pre' =p=> pre ->
+  post =p=> post' ->
+  prog_secure p pre post ->
+  prog_secure p pre' post'.
+Proof.
+  unfold prog_secure; intros.
+  apply H in H4.
+  specialize (H1 _ _ _ _ _ _ _ _ H2 H3 H4 H5).
+  intuition; repeat deex.
+  left.
+  do 6 eexists; intuition eauto.
+Qed.
+
+Definition read2 (a1 a2 : addr) :=
+  x <- Read a1;
+  y <- Read a2;
+  Ret (x, y).
+
+Theorem read2_secure:
+  forall (a1 a2:addr),
+  prog_secure (read2 a1 a2) (exists v1 v2, a1 |+> v1 * a2 |+> v2)%pred (exists v1 v2, a1 |+> v1 * a2 |+> v2)%pred.
+Proof.
+  unfold read2.
+
+  intros.
+  eapply bind_secure.
+  {
+    eapply pimpl_secure.
+    3: eapply frame_secure.
+    3: eapply read_secure.
+    instantiate (1 := (a2 |+>?)%pred).
+    cancel.
+    reflexivity.
+  }
+
+  intros.
+  eapply bind_secure.
+  {
+    eapply pimpl_secure.
+    3: eapply frame_secure.
+    3: eapply read_secure.
+    instantiate (1 := (a1 |+>?)%pred).
+    cancel.
+    reflexivity.
+  }
+
+  intros.
+  {
+    eapply pimpl_secure.
+    3: eapply frame_secure.
+    3: eapply ret_secure.
+    instantiate (1 := (a1 |+>? * a2 |+>?)%pred).
+    cancel.
+    cancel.
+  }
+Qed.
+
+Definition copy (a1 a2 : addr) :=
+  x <- Read a1;
+  Write a2 x.
+
+Theorem copy_secure:
+  forall (a1 a2:addr),
+  prog_secure (copy a1 a2) (exists v1 v2, a1 |+> v1 * a2 |+> v2)%pred
+                           (exists v1 v2, a1 |+> v1 * a2 |+> v2)%pred.
+Proof.
+  unfold copy.
+
+  intros.
+  eapply bind_secure.
+  {
+    eapply pimpl_secure.
+    3: eapply frame_secure.
+    3: eapply read_secure.
+    instantiate (1 := (a2 |+>?)%pred).
+    cancel.
+    reflexivity.
+  }
+
+  intros.
+  {
+    eapply pimpl_secure.
+    3: eapply frame_secure.
+    3: eapply write_secure.
+    instantiate (1 := (a1 |+>?)%pred).
+    cancel.
+    cancel.
+  }
+Qed.
+
+Theorem prog_secure_is_noninterference :
+  forall T (p : prog T) pre post a v1 v2 m1 m2 mp vm hm,
+  prog_secure p pre post ->
+  (a |+> v1 * diskIs mp)%pred m1 ->
+  (a |+> v2 * diskIs mp)%pred m2 ->
+  pre mp ->
+  forall m1' vm' hm' v,
+  exec m1 vm hm p (Finished m1' vm' hm' v) ->
+  exists m2' vm'' hm'',
+  exec m2 vm hm p (Finished m2' vm'' hm'' v).
+Proof.
+  unfold prog_secure; intros.
+  specialize (H _ _ _ _ _ _ _ _ H0 H1 H2 H3).
+  intuition; repeat deex; try congruence.
+  do 3 eexists.
+  inversion H4; subst.
+  eauto.
+Qed.
